Naming conventions per tipi. Varie

MasterThesis/Commons.lean
@@ -1,1 +1,1 @@
-abbrev ident := String
+abbrev Ident := String
