MasterThesis/LOOP/Interpreter.lean
@@ -2,14 +2,14 @@ import MasterThesis.LOOP.Language
 
 namespace LOOP
 
-open LOOP.com
+open LOOP.Com
 
-def eval (P : com) (σ : store) : store :=
+def eval (P : Com) (σ : Store) : Store :=
   match P with
   | SKIP    => σ
-  | ZER x   => store.update x 0 σ
-  | ASN x y => store.update x (σ y) σ
-  | INC x   => store.update x ((σ x) + 1) σ
+  | ZER x   => Store.update x 0 σ
+  | ASN x y => Store.update x (σ y) σ
+  | INC x   => Store.update x ((σ x) + 1) σ
   | SEQ P Q => (eval Q) (eval P σ)
   | FOR x P => (fun σ' => (eval P σ'))^[σ x] σ
 
