MasterThesis/LOOP/Language.lean
@@ -4,50 +4,50 @@ import MasterThesis.Commons
 
 namespace LOOP
 
-def store : Type := ident → Nat
+def Store : Type := Ident → Nat
 
-namespace store
+namespace Store
 
-def emp : store := fun _ => 0
+def emp : Store := fun _ => 0
 
-def update (x : ident) (v : Nat) (s : store) : store :=
-  fun (y : ident) => if x = y then v else (s y)
+def update (x : Ident) (v : Nat) (s : Store) : Store :=
+  fun (y : Ident) => if x = y then v else (s y)
 
 notation:100 "[" x:100 " ↦ " v:100 "]" s:100 => update x v s -- Migliorare?
 notation:100 "[" x:100 " ↦ " v:100 "]"       => [x ↦ v] emp -- Migliorare?
 
 @[simp]
-lemma update_same {s : store} {x y : ident} {v : Nat} : x = y → (store.update x v s) y = v := by
+lemma update_same {s : Store} {x y : Ident} {v : Nat} : x = y → (update x v s) y = v := by
   intros
   unfold update
   apply if_pos
   assumption
 
 @[simp]
-lemma update_other {s : store} {x y : ident} {v : Nat} : x ≠ y → (store.update x v s) y = (s y) := by
+lemma update_other {s : Store} {x y : Ident} {v : Nat} : x ≠ y → (update x v s) y = (s y) := by
   intros
   unfold update
   apply if_neg
   assumption
 
-lemma update_no_update {s : store} {x : ident} : (update x (s x) s) = s := by
+lemma update_no_update {s : Store} {x : Ident} : (update x (s x) s) = s := by
   funext y
   cases eq_or_ne x y with
   | inl /- x = y -/ => rw[update_same ‹x = y›, ‹x = y›]
   | inr /- x ≠ y -/ => rw[update_other ‹x ≠ y›]
 
-end store
+end Store
 
-inductive com : Type
-| SKIP : com
-| ZER : ident → com
-| ASN : ident → ident → com
-| INC : ident → com
-| SEQ : com → com → com
-| FOR : ident → com → com
+inductive Com : Type
+| SKIP : Com
+| ZER : Ident → Com
+| ASN : Ident → Ident → Com
+| INC : Ident → Com
+| SEQ : Com → Com → Com
+| FOR : Ident → Com → Com
 deriving Repr
 
-open com
+open Com
 
 infixl:80 ";;" => SEQ
 
