MasterThesis/SCORE/Language.lean
@@ -5,14 +5,14 @@ import MasterThesis.Commons
 
 namespace SCORE
 
-def store : Type := ident → List Int
+def Store : Type := Ident → List Int
 
-namespace store
+namespace Store
 
-def emp : store := fun _ => []
+def emp : Store := fun _ => []
 
-def update (x : ident) (l : List Int) (σ : store) : store :=
-  fun (y : ident) => if x = y then l else (σ y)
+def update (x : Ident) (l : List Int) (σ : Store) : Store :=
+  fun (y : Ident) => if x = y then l else (σ y)
 
 -- TODO: Migliorabile?
 notation:100 "[" x:100 " ↦ " l:100 "]" s:100 => update x l s
@@ -21,26 +21,26 @@ notation:100 "[" x:100 " ↦ " l:100 "]"       => [x ↦ l] emp
 #eval (["z" ↦ [3]] ["y" ↦ [2]] ["x" ↦ [1]]) "x"
 
 @[simp]
-lemma update_same {σ : store} {x y : ident} {l : List Int} : x = y → (store.update x l σ) y = l := by
+lemma update_same {σ : Store} {x y : Ident} {l : List Int} : x = y → (update x l σ) y = l := by
   intros; simp only [if_pos ‹x = y›, update]
 
 @[simp]
-lemma update_other {σ : store} {x y : ident} {l : List Int} : x ≠ y → (store.update x l σ) y = σ y := by
+lemma update_other {σ : Store} {x y : Ident} {l : List Int} : x ≠ y → (update x l σ) y = σ y := by
   intros; simp only [if_neg ‹x ≠ y›, update]
 
-lemma update_shrink {σ : store} {x : ident} {l₁ l₂ : List Int} : (store.update x l₂ (store.update x l₁ σ)) = store.update x l₂ σ := by
+lemma update_shrink {σ : Store} {x : Ident} {l₁ l₂ : List Int} : (update x l₂ (update x l₁ σ)) = update x l₂ σ := by
   funext y
   cases eq_or_ne x y with
   | inl /- x = y -/ => simp only [update_same ‹x = y›]
   | inr /- x ≠ y -/ => simp only [update_other ‹x ≠ y›]
 
-lemma update_unchanged {σ : store} {x : ident} : store.update x (σ x) σ = σ := by
+lemma update_unchanged {σ : Store} {x : Ident} : update x (σ x) σ = σ := by
   funext y
   cases eq_or_ne x y with
   | inl /- x = y -/ => rewrite [‹x = y›]; simp only [update_same]
   | inr /- x ≠ y -/ => simp only [update_other ‹x ≠ y›]
 
-lemma update_unchanged_cons {σ : store} {x : ident} {v : Int} : (σ x).head? = some v → store.update x (v :: (σ x).tail) σ = σ := by
+lemma update_unchanged_cons {σ : Store} {x : Ident} {v : Int} : (σ x).head? = some v → update x (v :: (σ x).tail) σ = σ := by
   intro
   funext y
   cases eq_or_ne x y with
@@ -55,33 +55,38 @@ lemma update_unchanged_cons {σ : store} {x : ident} {v : Int} : (σ x).head? = 
     have : ([x ↦ (v :: (σ x).tail)] σ) y = σ y := by
       { simp [‹x ≠ y›] }; rw [this]
 
-end store
+end Store
 
-inductive state : Type :=
-| prog : store → state
+inductive State : Type :=
+| prog : Store → State
 | fail
 
-notation "⊥" => state.fail
+notation "⊥" => State.fail
 
-namespace state
+namespace State
 
-end state
+lemma prog_or_bot (s : State) : (∃ (σ : Store), s = prog σ) ∨ s = ⊥ := by
+  cases s
+  case prog σ => left; exact ⟨σ, rfl⟩
+  case fail   => right; rfl
 
-inductive com : Type
-| SKIP : com
-| CON  : ident → com
-| NOC  : ident → com
-| DEC  : ident → com
-| INC  : ident → com
-| SEQ  : com → com → com
-| FOR  : ident → com → com
+end State
+
+inductive Com : Type
+| SKIP : Com
+| CON  : Ident → Com
+| NOC  : Ident → Com
+| DEC  : Ident → Com
+| INC  : Ident → Com
+| SEQ  : Com → Com → Com
+| FOR  : Ident → Com → Com
 deriving Repr
 
-open com
+open Com
 
 infixl:80 ";;" => SEQ
 
-def inv (P : com) : com :=
+def inv (P : Com) : Com :=
   match P with
   | SKIP    => SKIP
   | CON x   => NOC x
@@ -93,7 +98,7 @@ def inv (P : com) : com :=
 
 postfix:max "⁻¹" => inv
 
-theorem inv_inv (P : com) : (inv (inv P)) = P := by
+theorem inv_inv (P : Com) : (inv (inv P)) = P := by
   induction  P
   case SKIP        => simp[inv]
   case CON         => simp[inv]
