MasterThesis/LOOP/Functions.lean
@@ -2,12 +2,12 @@ import MasterThesis.LOOP.Language
 
 namespace LOOP.func
 
-open LOOP LOOP.com
+open LOOP LOOP.Com
 
 /- Somma tra due numeri
    {x = a, y = b, z = 0}
 -/
-def sum : com :=
+def sum : Com :=
   FOR "x" (INC "z") ;;
   FOR "y" (INC "z")
 -- {x = a, y = b, z = a + b}
@@ -15,11 +15,12 @@ def sum : com :=
 /- Predecessore di un numero
    {x = ?, y = a, z = 0}
 -/
-def pred : com :=
+def pred : Com :=
   FOR "y" (
     ZER "x" ;;
     FOR "z" (INC "x") ;;
     INC "z"
   )
 -- {x = a - 1, y = a, z = a}
+
 end LOOP.func
