MasterThesis/SCORE/Functions.lean
@@ -2,31 +2,28 @@ import MasterThesis.SCORE.Language
 
 namespace SCORE.func
 
-open SCORE SCORE.com
+open SCORE SCORE.Com
 
 /- Somma tra due numeri
    {x = a, y = b, z = 0} -/
-def sum : com :=
+def sum : Com :=
   FOR "x" (INC "z") ;;
   FOR "y" (INC "z")
 -- {x = a, y = b, z = a + b}
 
 /- Differenza tra due numeri
    {x = a, y = b, z = 0} -/
-def diff : com :=
+def diff : Com :=
   FOR "x" (INC "z") ;;
   FOR "y" (DEC "z")
 -- {x = a, y = b, z = a - b}
 
 /- Prodotto tra due numeri
    {x = a, y = b, z = 0} -/
-def prod : com :=
+def prod : Com :=
    FOR "y" (
       FOR "x" (INC "z")
    )
 -- {x = a, y = b, z = a * b}
-
-def store0 : store := ["x" ↦ [1]] ["y" ↦ [2]] ["z" ↦ [0]]
-def store1 : store := ["x" ↦ [-1]] ["y" ↦ [-2]] ["z" ↦ [0]]
 
 end SCORE.func
