MasterThesis/SCORE/Test/Compiler.lean
@@ -1,11 +1,11 @@
 import MasterThesis.LOOP.Functions
-import MasterThesis.SCORE.Compiler
+import MasterThesis.SCORE.Compiler_v1
 
 open SCORE
 
-def store0 : store := ["x" ↦ [0]] ["y" ↦ [3]] ["z" ↦ [0]]
+def store0 : Store := ["x" ↦ [0]] ["y" ↦ [3]] ["z" ↦ [0]]
 
-def storePred : store := (eval (L2S LOOP.func.pred) store0)
+def storePred : Store := (eval (L2S LOOP.func.pred) store0)
 #eval  storePred "x"
-def storePredᵢ : store := (evalI (L2S LOOP.func.pred) storePred)
+def storePredᵢ : Store := (evalI (L2S LOOP.func.pred) storePred)
 #eval storePredᵢ "y"
